\documentclass[12pt, letterpaper,bibtotoc, tablecaptionabove, figurecaptionabove]{article}

%%%%

\setlength{\headheight}{10pt}
\setlength{\headsep}{15pt}
\setlength{\topmargin}{-25pt}
\setlength{\topskip}{0in}
\setlength{\textheight}{8.7in}
\setlength{\footskip}{0.3in}
\setlength{\oddsidemargin}{0.0in}
\setlength{\evensidemargin}{0.0in}
\setlength{\textwidth}{6.5in}

\usepackage{setspace}
\setstretch{1.1}
\setlength{\parskip}{5pt}%{6pt}
\setlength{\parindent}{5pt}
\usepackage[margin=.85in]{geometry}
\usepackage{subfiles}
\usepackage{xcolor}
\usepackage{bbm}
\usepackage{graphicx}
\graphicspath{{images/}{../images/}}
\usepackage{amsmath}
\usepackage{amssymb}
\usepackage{multicol}
\usepackage{amsthm}
\usepackage{enumerate}
\newtheorem{proposition}{Proposition}
\newtheorem{definition}{Definition}
\newtheorem{remark}{Remark}
\newtheorem{lemma}{\ellemma}
\newtheorem{notation}{Notation}
\newtheorem{corollary}{Corollary}
\newcommand{\norm}[1]{\left\lVert#1\right\rVert}

%\usepackage{fontspec}
%\setmainfont{book antiqua}

\usepackage{bm}

\usepackage[utf8]{inputenc}
\usepackage[english]{babel}
\usepackage{hyperref}
\hypersetup{
    colorlinks=true,
    linkcolor=blue,
    citecolor=red,
}



%%%%

\begin{document}


\title{\bf{''DSGE''}\\  Problem Set 1}
%\subtitle{Take Home Exam}
\author{ Sofonias Alemu Korsaye}
%\date{07/02/2017}
\maketitle


\begin{enumerate}
\item{\bf{Exercise 1}}
\begin{eqnarray*}
\begin{aligned}
&\frac{1}{e^{z_{t}} k_{t}^{\alpha}-Ae^{z_t}k_t^\alpha}=
\beta E_{t}\left\{\frac{\alpha e^{z_{t+1}} k_{t+1}^{\alpha-1}}{e^{z_{t+1}} k_{t+1}^{\alpha}-Ae^{z_{t+1}}k_{t+1}^\alpha}\right\}\\
&\frac{1}{e^{z_{t}} k_{t}^{\alpha}-Ae^{z_t}k_t^\alpha}=\frac{\beta \alpha}{k_{t+1}(1-A)}\\
&\frac{1}{e^{z_{t}} k_{t}^{\alpha}(1-A)}=\frac{\beta \alpha}{k_{t+1}(1-A)}\\
&k_{t+1}=A e^{z_t}k_t^\alpha, \text{ where } A=\beta \alpha \ .
\end{aligned}
\end{eqnarray*}
\item{\bf{Exercise 2}}
\begin{eqnarray*}
\begin{aligned}
&c_{t}=(1-\tau)\left[w_{t} \ell_{t}+\left(r_{t}-\delta\right) k_{t}\right]+k_{t}+T_{t}-k_{t+1}\\
&1/c_t=\beta E_{t}\left\{1/c_{t+1}\left[\left(r_{t+1}-\delta\right)(1-\tau)+1\right]\right\}\\
&-\frac{a}{1-\ell_t}=\frac{1}{c_t} w_{t}(1-\tau)\\
&r_t=\alpha e^{z_t}k_t^{\alpha-1}\ell_t^{1-\alpha} \\
& w_t=(1-\alpha)e^{z_t}k_t^\alpha \ell_t^{-\alpha} \\ 
&{\tau\left[w_{t} \ell_{t}+\left(r_{t}-\delta\right) k_{t}\right]=T_{t}} \\ 
\end{aligned}
\end{eqnarray*}
\item{\bf{Exercise 3}}
\begin{eqnarray*}
\begin{aligned}
&c_{t}=(1-\tau)\left[w_{t} \ell_{t}+\left(r_{t}-\delta\right) k_{t}\right]+k_{t}+T_{t}-k_{t+1}\\
&c_t^{-\gamma}=\beta E_{t}\left\{1/c_{t+1}\left[\left(r_{t+1}-\delta\right)(1-\tau)+1\right]\right\}\\
&-\frac{a}{1-\ell_t}=c_t^{-\gamma} w_{t}(1-\tau)\\
&r_t=\alpha e^{z_t}k_t^{\alpha-1}\ell_t^{1-\alpha} \\
& w_t=(1-\alpha)e^{z_t}k_t^\alpha \ell_t^{-\alpha} \\ 
&{\tau\left[w_{t} \ell_{t}+\left(r_{t}-\delta\right) k_{t}\right]=T_{t}} \\ 
\end{aligned}
\end{eqnarray*}

\item{\bf{Exercise 4}}
\begin{eqnarray*}
\begin{aligned}
&c_{t}=(1-\tau)\left[w_{t} \ell_{t}+\left(r_{t}-\delta\right) k_{t}\right]+k_{t}+T_{t}-k_{t+1}\\
&c_t^{-\gamma}=\beta E_{t}\left\{1/c_{t+1}\left[\left(r_{t+1}-\delta\right)(1-\tau)+1\right]\right\}\\
&-a(1-\ell_t)^{-\xi}=c_t^{-\gamma} w_{t}(1-\tau)\\
&r_t=\frac{e^{z_t}}{\eta}(\alpha k_t^\eta+(1-\alpha)\ell_t^\eta)^{\frac{1}{\eta}-1}\alpha\eta k_t^{\eta-1} \\
& w_t=\frac{e^{z_t}}{\eta}(\alpha k_t^\eta+(1-\alpha)\ell_t^\eta)^{\frac{1}{\eta}-1}(1-\alpha)\eta \ell_t^{\eta-1} \\ 
&{\tau\left[w_{t} \ell_{t}+\left(r_{t}-\delta\right) k_{t}\right]=T_{t}} \\ 
\end{aligned}
\end{eqnarray*}

\item{\bf{Exercise 5}}

\begin{eqnarray*}
\begin{aligned}
&c_{t}=(1-\tau)\left[w_{t}+\left(r_{t}-\delta\right) k_{t}\right]+k_{t}+T_{t}-k_{t+1}\\
&c_t^{-\gamma}=\beta E_{t}\left\{c_{t+1}^{-\gamma}\left[\left(r_{t+1}-\delta\right)(1-\tau)+1\right]\right\}\\
&r_t=\alpha k_t^{\alpha-1}(e^{z_t})^{1-\alpha} \\
& w_t=k_t^\alpha e^{z_t}(1-\alpha)(e^{z_t})^{-\alpha}\\ 
&{\tau\left[w_{t} +\left(r_{t}-\delta\right) k_{t}\right]=T_{t}} \\ 
\end{aligned}
\end{eqnarray*}
The steady state is given by the variables $\{c,k,w,r,\tau\}$ that solve the following system of equations.
\begin{eqnarray*}
\begin{aligned}
&c=(1-\tau)\left[w+\left(r-\delta\right) k\right]+T\\
&c^{-\gamma}=\beta E\left\{c^{-\gamma}\left[\left(r-\delta\right)(1-\tau)+1\right]\right\}\\
&r=\alpha k^{\alpha-1}(e^{z})^{1-\alpha} \\
 &w=k^\alpha e^{z}(1-\alpha)(e^{z})^{-\alpha}\\ 
&{\tau\left[w+\left(r-\delta\right) k\right]=T} \\ 
\end{aligned}
\end{eqnarray*}

The above described sustem can be analytically solved. The solutions are given by
\begin{eqnarray*}
\begin{aligned}
&r=\frac{1-\beta}{\beta(1-\tau)}+\delta\\
&k=\left(\frac{r}{\alpha}\right)^{\frac{1}{\alpha-1}}\\
&w=k^\alpha(1-\alpha)\\
&c=w+(r-\delta)*k\\
&T=\tau(w+(r-\delta)*k)\\
\end{aligned}
\end{eqnarray*}




\item{\bf{Exercise 6}}

\begin{eqnarray*}
\begin{aligned}
&c_{t}=(1-\tau)\left[w_{t} \ell_{t}+\left(r_{t}-\delta\right) k_{t}\right]+k_{t}+T_{t}-k_{t+1}\\
&c_t^{-\gamma}=\beta E_{t}\left\{c_{t+1}^{-\gamma}\left[\left(r_{t+1}-\delta\right)(1-\tau)+1\right]\right\}\\
&-a(1-\ell_t)^{-\xi}=c_t^{-\gamma} w_{t}(1-\tau)\\
&r_t=\alpha k_t^{\alpha-1}(\ell_t e^{z_t})^{1-\alpha} \\
& w_t=k_t^\alpha e^{z_t}(1-\alpha)(\ell_t e^{z_t})^{-\alpha}\\ 
&{\tau\left[w_{t} \ell_{t}+\left(r_{t}-\delta\right) k_{t}\right]=T_{t}} \\ 
\end{aligned}
\end{eqnarray*}
The steady state is given by the variables $\{c,k,\ell,w,r,\tau,z\}$ that solve the following system of equations.

\begin{eqnarray*}
\begin{aligned}
&c=(1-\tau)\left[w\ell+\left(r-\delta\right) k\right]+k+T-k\\
&1=\beta \left\{\left(r-\delta\right)(1-\tau)+1\right\}\\
-&a(1-\ell)^{-\xi}=c_t^{-\gamma} w(1-\tau)\\
&r=\alpha k^{\alpha-1}(\ell_t e^{z})^{1-\alpha} \\
 &w=k^\alpha e^{z}(1-\alpha)(\ell e^{z})^{-\alpha}\\ 
&{\tau\left[w \ell+\left(r-\delta\right) k\right]=T} \\ 
\end{aligned}
\end{eqnarray*}



\end{enumerate}










\end{document}